support for polymorphic intrinsics

Examples/poly.ml
@@ -1,0 +1,10 @@
+open Mica
+(* Polymorphic intrinsics: identity instantiated at different types. *)
+
+(* [Fun.id : 'a -> 'a] at int. *)
+let id_int (x : int) : int = Fun.id x
+[@@spec fun x -> ret (fun v -> assert (v = x))];;
+
+(* The same [Fun.id] at string: one symbol, a different instantiation. *)
+let id_str (s : string) : string = Fun.id s
+[@@spec fun s -> ret (fun v -> assert (String.equal v s))];;
